add relational ranking rules

Lentil/Util.lean
@@ -8,6 +8,152 @@ def binderIdentToFunBinder (stx : TSyntax ``binderIdent) : MacroM (TSyntax ``Par
   | `(binderIdent| _ ) =>  `(Parser.Term.funBinder| _ )
   | _ => Macro.throwUnsupported
 
+theorem List.mem_forall_iff_fin_index {α : Type u} (l : List α) (p : α → Prop) :
+  (∀ x, x ∈ l → p x) ↔ ∀ (x : Fin l.length), p l[x] := by
+  constructor
+  · intro h x ; apply h ; simp
+  · intro h x hin ; rw [List.mem_iff_getElem] at hin
+    rcases hin with ⟨n, hlt, heq⟩ ; subst_vars ; exact h ⟨_, hlt⟩
+
+theorem List.mem_exists_iff_fin_index {α : Type u} (l : List α) (p : α → Prop) :
+  (∃ x, x ∈ l ∧ p x) ↔ ∃ (x : Fin l.length), p l[x] := by
+  constructor
+  · intro ⟨x, hin, h⟩ ; rw [List.mem_iff_getElem] at hin
+    rcases hin with ⟨n, hlt, heq⟩ ; subst_vars ; exists ⟨_, hlt⟩
+  · intro ⟨n, h⟩ ; exists l[n] ; simp ; try assumption
+
+theorem List.finRange_fin_in (n : Nat) : ∀ (x : Fin n), x ∈ List.finRange n := by
+  intro ⟨x, hlt⟩ ; rw [List.mem_iff_getElem] ; simp ; assumption
+
+-- sometimes we depend on theorems that themselves or similar ones
+-- are present in Mathlib, but to reduce dependencies, we prove them here
+
+-- NOTE: usually, the unification is not strong enough to figure out `p`,
+-- which would be supplied by the user in practice
+theorem Nat.find_min {p : Nat → Prop} (n : Nat) (h : p n) :
+  ∃ n', n' ≤ n ∧ p n' ∧ ∀ m, m < n' → ¬ p m := by
+  induction n using Nat.strongRecOn
+  rename_i n ih
+  by_cases h' : ∃ m, m < n ∧ p m
+  · rcases h' with ⟨m, hlt, h'⟩
+    have ⟨n', hle, ha, hb⟩ := ih _ hlt h'
+    exists n' ; apply And.intro (by omega) (And.intro ‹_› ‹_›)
+  · simp at h' ; exists n ; simp_all
+
+theorem Nat.find_min' {p : Nat → Prop} (n : Nat) (h : p n) :
+  ∃ n', n' ≤ n ∧ p n' ∧ ∀ m, p m → n' ≤ m := by
+  have ⟨n', hn', ha, hb⟩ := Nat.find_min _ h
+  exists n' ; apply And.intro ‹_› (And.intro ‹_› _) ; intros ; apply Nat.le_of_not_lt ; intro hlt ; solve_by_elim
+
+-- NOTE: the following part about induction on lists of natural numbers w.r.t. lexicographic order
+-- is potentially in Lean (but not in the `main` branch), so here we just prove things
+-- as we need
+
+namespace NatListLex
+
+section Main
+
+universe u
+variable {α : Type u} {n : Nat} (r : α → α → Prop) (rl : { l : List α // l.length = n } → { l : List α // l.length = n } → Prop)
+
+/-- Given a list whose length is `n + 1`, return its head and tail
+    and also an associated proof. -/
+def List.succLengthInv (lo : { l : List α // l.length = n.succ }) :
+  PSigma fun a => { l : List α // l.length = n ∧ lo.val = a :: l } :=
+  match lo with
+  | ⟨a :: l, h⟩ => ⟨a, ⟨l, And.intro (Nat.succ_inj'.mp h) rfl⟩⟩
+  | ⟨[], h⟩ => by simp at h
+
+/-- Just like `Prod.Lex`, but defined over the `(head, tail)` pairs
+    of lists. -/
+def List.consLex (l1 l2 : { l : List α // l.length = n.succ }) : Prop :=
+  match List.succLengthInv l1, List.succLengthInv l2 with
+  | ⟨x, ⟨l1, h1⟩⟩, ⟨y, ⟨l2, h2⟩⟩ => Prod.Lex r rl (x, ⟨l1, h1.1⟩) (y, ⟨l2, h2.1⟩)
+
+-- adapted from `Prod.lexAccessible`
+theorem consLexAccessible (aca : Acc r a) (acl : ∀ (b : { l : List α // l.length = n }), Acc rl b)
+    (l : { l : List α // l.length = n }) :
+  Acc (List.consLex r rl) (⟨a :: l.val, congrArg Nat.succ l.property⟩ : { l : List α // l.length = n.succ }) := by
+  induction aca generalizing l with
+  | intro xa _ iha =>
+    induction (acl l) with
+    | intro xl _ ihl =>
+      apply Acc.intro
+      intro ⟨l', hl'⟩ hlt
+      rcases l' with _ | ⟨x', l'⟩ <;> simp at hl'
+      simp [List.consLex] at hlt
+      cases hlt with
+      | left  _ _ h => simp [List.succLengthInv] at h ; apply iha _ h ⟨_, hl'⟩
+      | right _ h   => simp [List.succLengthInv] at h ; apply ihl _ h
+
+end Main
+
+def List.cons_wfRel {α : Type u} {n : Nat} (h : WellFoundedRelation α)
+  (hl : WellFoundedRelation { l : List α // l.length = n }) :
+  WellFoundedRelation { l : List α // l.length = n.succ } where
+  rel := List.consLex h.rel hl.rel
+  wf := ⟨fun l =>
+    match List.succLengthInv l with
+    | ⟨a, ⟨l', hh⟩⟩ => (congrArg (Acc _) ((Subtype.eq (a1 := ⟨a :: l', _⟩) hh.2.symm))) ▸
+      consLexAccessible _ _ (WellFounded.apply h.wf a) (WellFounded.apply hl.wf) ⟨l', hh.1⟩⟩
+
+def List.natLexLt_wfRel (n : Nat) : WellFoundedRelation { l : List Nat // l.length = n } :=
+  match n with
+  | .zero => emptyWf
+  | .succ n' => List.cons_wfRel Nat.lt_wfRel (List.natLexLt_wfRel n')
+
+def List.natLexLt : List Nat → List Nat → Prop
+  | x :: xs, y :: ys => x < y ∨ (x = y ∧ natLexLt xs ys)
+  | _, _ => False
+
+/-- An equivalent way of expressing `List.natLexLt`. -/
+def List.natLexLt' (l l' : List Nat) : Prop :=
+  ∃ (i : Nat) (hlt : i < l.length) (hlt' : i < l'.length),
+    l.take i = l'.take i ∧ l[i]'hlt < l'[i]'hlt'
+
+theorem List.natLexLt_alt (l l' : List Nat) :
+  List.natLexLt l l' ↔ List.natLexLt' l l' := by
+  induction l generalizing l' with
+  | nil => simp [List.natLexLt, List.natLexLt']
+  | cons x l ih =>
+    cases l' with
+    | nil => simp [List.natLexLt, List.natLexLt']
+    | cons y l' =>
+      simp [List.natLexLt, List.natLexLt', ih] ; constructor
+      · intro h ; cases h with
+        | inl h => exists 0 ; simp ; assumption
+        | inr h =>
+          rcases h with ⟨heq, i, h⟩
+          subst y ; exists (i + 1) ; simp ; exact h
+      · intro ⟨i, htakeeq, h⟩
+        cases i with
+        | zero => simp at h ; apply Or.inl h
+        | succ i =>
+          simp at htakeeq h ; right ; apply And.intro htakeeq.1
+          exists i ; apply And.intro htakeeq.2 h
+
+-- the underlying `rel` of `List.natLexLt_wfRel` is `List.natLexLt`
+theorem List.natLexLt_wfRel_rel (n : Nat) l l' :
+  (List.natLexLt_wfRel n |>.rel l l') ↔ List.natLexLt l.val l'.val := by
+  rcases l with ⟨l, hl⟩ ; rcases l' with ⟨l', hl'⟩
+  induction n generalizing l l' with
+  | zero => simp at hl hl' ; subst_vars ; simp [List.natLexLt_wfRel, emptyWf, List.natLexLt, emptyRelation]
+  | succ n' ih =>
+    rcases l with _ | ⟨x, l⟩ <;> simp at hl
+    rcases l' with _ | ⟨y, l'⟩ <;> simp at hl'
+    simp [List.natLexLt_wfRel, List.cons_wfRel, List.consLex, List.succLengthInv, List.natLexLt, Nat.lt_wfRel, Prod.lex_def, ih]
+
+noncomputable def List.natLexRecOn
+    {motive : List Nat → Sort u}
+    (l : List Nat)
+    (ind : ∀ l, (∀ l', l'.length = l.length → List.natLexLt l' l → motive l') → motive l) : motive l :=
+  (List.natLexLt_wfRel l.length |>.wf.fix)
+    (fun ⟨l', hl'⟩ (recc : ∀ (l_' : { l_ : List Nat // l_.length = l.length }), _ → motive l_') =>
+      ind l' (fun l'' hl'' hlt =>
+        recc ⟨l'', Eq.trans hl'' hl'⟩ ((List.natLexLt_wfRel_rel l.length ⟨l'', Eq.trans hl'' hl'⟩ ⟨l', hl'⟩ |>.mpr) hlt))) ⟨l, rfl⟩
+
+end NatListLex
+
 register_option lentil.pp.useDelab : Bool := {
   defValue := true
   descr := "Use Delab instead of Unexpander for delaboration. "
@@ -18,6 +164,7 @@ register_option lentil.pp.autoRenderSatisfies : Bool := {
   descr := "Automatically render an application `p e` as `e |=tla= p` when `p` is a TLA formula. "
 }
 
+register_simp_attr tla_nontemporal_def  -- marking the non-temporal parts of TLA
 register_simp_attr tlasimp_def
 register_simp_attr tlasimp
 register_simp_attr tladual      -- experimental
